steel/Zeta.Steel.ExternalPtr.fsti
@@ -14,8 +14,8 @@ val extern_ptr : Type0
 [@@erasable]
 noeq
 type state =
-| Unread: (out_len: U32.t) -> state
-| Read: (out_len: U32.t) -> state
+| Unread: (out_len: SizeT.t) -> state
+| Read: (out_len: SizeT.t) -> state
 | Written: (written: Seq.seq U8.t) -> state
 
 val extern_in_out_pts_to (e1: extern_ptr) (e2: extern_ptr) (in_contents: Seq.seq U8.t) (s: state) : vprop
@@ -23,29 +23,29 @@ val extern_in_out_pts_to (e1: extern_ptr) (e2: extern_ptr) (in_contents: Seq.seq
 [@@__reduce__]
 let is_valid_state_true
   (e1: extern_ptr)
-  (n1: U32.t)
+  (n1: SizeT.t)
   (e2: extern_ptr)
-  (n2: U32.t)
+  (n2: SizeT.t)
 : Tot vprop
 = exists_ (fun in_contents ->
     extern_in_out_pts_to e1 e2 in_contents (Unread n2) `star`
-    pure (U32.v n1 == Seq.length in_contents)
+    pure (SizeT.v n1 == Seq.length in_contents)
   )
 
 let is_valid_state
   (e1: extern_ptr)
-  (n1: U32.t)
+  (n1: SizeT.t)
   (e2: extern_ptr)
-  (n2: U32.t)
+  (n2: SizeT.t)
   (b: bool)
 : Tot vprop
 = if b then is_valid_state_true e1 n1 e2 n2 else emp
 
 val extern_in_out_pts_to_is_valid
   (e1: extern_ptr)
-  (n1: U32.t)
+  (n1: SizeT.t)
   (e2: extern_ptr)
-  (n2: U32.t)
+  (n2: SizeT.t)
 : STT bool
   emp
   (fun b -> is_valid_state e1 n1 e2 n2 b)
@@ -55,16 +55,16 @@ val copy_extern_input_ptr
   (e1: extern_ptr)
   (w1: Ghost.erased (Seq.seq U8.t))
   (e2: extern_ptr)
-  (n: U32.t)
-  (out_len: Ghost.erased U32.t)
+  (n: SizeT.t)
+  (out_len: Ghost.erased SizeT.t)
   (a: A.array U8.t)
 : ST unit
     (extern_in_out_pts_to e1 e2 w1 (Unread out_len) `star` exists_ (fun contents -> A.pts_to a full_perm contents))
     (fun _ ->
       extern_in_out_pts_to e1 e2 w1 (Read out_len) `star` A.pts_to a full_perm w1
     )
-    (A.length a == U32.v n /\
-      Seq.length w1 == U32.v n)
+    (A.length a == SizeT.v n /\
+      Seq.length w1 == SizeT.v n)
     (fun _ -> True)
 
 inline_for_extraction
@@ -72,7 +72,7 @@ val copy_extern_output_ptr
   (e1: extern_ptr)
   (w1: Ghost.erased (Seq.seq U8.t))
   (e2: extern_ptr)
-  (n: U32.t)
+  (n: SizeT.t)
   (a: A.array U8.t)
   (p: perm)
   (contents: Ghost.erased (Seq.seq U8.t))
@@ -81,5 +81,5 @@ val copy_extern_output_ptr
     (fun _ ->
       extern_in_out_pts_to e1 e2 w1 (Written contents) `star` A.pts_to a p contents
     )
-    (A.length a == U32.v n)
+    (A.length a == SizeT.v n)
     (fun _ -> True)
