steel/Zeta.Steel.Util.fst
@@ -68,28 +68,10 @@ let update_if (b:bool) (default_ upd_: 'a)
   : 'a
   = if b then upd_ else default_
 
-// let next (t:U64.t)
-//   : option U64.t
-//   = let ctr = FStar.Int.Cast.uint64_to_uint32 t in
-//     if FStar.UInt.fits (U32.v ctr + 1) 32
-//     then Some (U64.add t 1uL)
-//     else None
+let wrap_platform32_check (_:unit)
+  : STT (squash (FStar.SizeT.fits_u32)) emp (fun _ -> emp)
+  = Steel.ST.HigherArray.intro_fits_u32()
 
-// let will_add_overflow32 (x y:U32.t)
-//   : res:bool{
-//        res <==> not (FStar.UInt.fits (U32.v x + U32.v y) 32)
-//     }
-//   = let open U32 in
-//     (0xfffffffful -^ x) <^ y
-
-// module C = FStar.Int.Cast
-
-// let try_increment_counter (x:U64.t)
-//   : Tot (v:option (U64.t) { v == next x })
-//   = let ctr = FStar.Int.Cast.uint64_to_uint32 x in
-//     if will_add_overflow32 ctr 1ul
-//     then None
-//     else let res = U64.(x +^ 1uL) in
-//          Some res
-
-       
+#push-options "--warn_error -272" //intentional top-level effect here
+let fits_u32 : squash (FStar.SizeT.fits_u32) = wrap_platform32_check()
+#pop-options
