steel/Zeta.Steel.VerifierTypes.fst
@@ -132,10 +132,11 @@ let elim_thread_state_inv (#o:_) (#tsm:M.thread_state_model) (t:thread_state_t)
   = elim_pure _
 module Cast = FStar.Int.Cast
 
-let as_u32 (s:U16.t) : U32.t = Cast.uint16_to_uint32 s
+inline_for_extraction
+let as_size_t (s:U16.t) : SizeT.t = SizeT.mk_u32 (Cast.uint16_to_uint32 s)
 
 let read_store #tsm t slot =
-  let se_opt = A.read t.store (as_u32 slot) in
+  let se_opt = A.read t.store (as_size_t slot) in
   match se_opt with
   | None -> return None
   | Some (se : M.store_entry) ->
@@ -143,11 +144,11 @@ let read_store #tsm t slot =
                     value = se.value }))
 
 let write_store #tsm t slot v =
-  let se_opt = A.read t.store (as_u32 slot) in
+  let se_opt = A.read t.store (as_size_t slot) in
   match se_opt with
   | Some (se : M.store_entry) ->
     let se' = { se with value = v } in
-    A.write t.store (as_u32 slot) (Some se');
+    A.write t.store (as_size_t slot) (Some se');
     return ()
 
 let restore_thread_state_inv_app #_ #tsm t app_results processed_entries =
